theories/simulang/na_inv/adequacy.v
@@ -64,25 +64,27 @@ Proof.
   iIntros (? gs Hgs) "_ _ _ _ !#".
   iSplit. { iApply big_sepM_intro. iIntros "!>" (???). iApply val_wf_sound. by apply: Hgs. }
   rewrite /prog_rel.
-  iIntros "!# %f %arg %body".
+  iIntros "!# %f %fn".
   iDestruct (Hrel _) as "Hrel". clear Hrel.
   destruct (decide (f = fname)) as [->|Hne].
   - rewrite !lookup_insert.
-    iIntros ([= <- <-]). iExists _, _. iSplitR; first done.
+    iIntros ([= <-]). iExists _. iSplitR; first done.
     (* TODO Factor this into a general lemma? *)
     iIntros (v_t v_s π) "[Hc #Hval] /=".
     iApply (sim_wand with "[Hc]").
-    + iApply (gen_log_rel_singleton with "[Hrel] Hval [Hc]"); first done.
+    + rewrite /apply_func /= -!subst_map_singleton.
+      iApply (gen_log_rel_singleton with "[Hrel] Hval [Hc]"); first done.
       * by iApply log_rel_ctx.
       * done.
     + simpl. iIntros (??). auto.
   - rewrite !lookup_insert_ne //.
-    iIntros (Hf). iExists arg, body. iSplit; first done.
+    iIntros (Hf). iExists fn. destruct fn as [arg body]. iSplit; first done.
     specialize (Hpwf _ _ Hf). destruct Hpwf as [HKwf HKclosed].
     (* TODO Factor this into a lemma? *)
     iIntros (v_t v_s π) "[Hc #Hval] /=".
     iApply (sim_wand with "[Hc]").
-    + iApply (gen_log_rel_singleton with "[Hrel] Hval [Hc]"); first set_solver.
+    + rewrite /apply_func /= -!subst_map_singleton.
+      iApply (gen_log_rel_singleton with "[Hrel] Hval [Hc]"); first set_solver.
       * by iApply log_rel_refl.
       * done.
     + simpl. iIntros (??). auto.
